proof/invariants/UpdateShadow1Structure.v
@@ -1,5 +1,5 @@
  (*******************************************************************************)
-(*  © Université Lille 1, The Pip Development Team (2015-2017)                 *)
+(*  © Université Lille 1, The Pip Development Team (2015-2018)                 *)
 (*                                                                             *)
 (*  This software is a computer program whose purpose is to run a minimal,     *)
 (*  hypervisor relying on proven properties such as memory isolation.          *)
@@ -6089,6 +6089,650 @@ unfold consistency in *;intuition.
     cbn;trivial. 
     }
 Qed.
+Lemma physicalPageNotDerivedRemoveVaddr    
+entry s descChild vaChild currentPart level
+     idxDescChild ptDescChild currentPD ptDescChildFromPD idxDescChild1
+     phyDescChild pdChildphy idxvaChild ptVaChildpd shadow1Child
+     ptVaChildFromSh1 vainve sh2Childphy ptVaChildsh2 vainparent defautvaddr
+     currentShadow ptVaInCurPart:
+ propagatedPropertiesRemoveVaddr s descChild vaChild currentPart level
+     idxDescChild ptDescChild currentPD ptDescChildFromPD idxDescChild1
+     phyDescChild pdChildphy idxvaChild ptVaChildpd shadow1Child
+     ptVaChildFromSh1 vainve sh2Childphy ptVaChildsh2 vainparent defautvaddr
+     currentShadow ptVaInCurPart (StateLib.getIndexOfAddr vainparent fstLevel) false
+     false  -> 
+isPartitionFalse ptVaInCurPart
+       (StateLib.getIndexOfAddr vainparent fstLevel) s -> 
+lookup ptVaInCurPart (StateLib.getIndexOfAddr vainparent fstLevel)
+            (memory s) beqPage beqIndex = Some (VE entry)  
+->  getPDFlag currentShadow vainparent s = false -> 
+   (exists pagetoremove : page,
+      getAccessibleMappedPage currentPD s vainparent = SomePage pagetoremove /\
+      (forall child : page,
+       In child (getChildren currentPart s) ->
+       ~ In pagetoremove (getMappedPages child s))) -> 
+(* ~ isDerived (currentPartition s) vainparent s ->  *)
+physicalPageNotDerived s ->
+physicalPageNotDerived
+  {|
+  currentPartition := currentPartition s;
+  memory := add ptVaInCurPart (StateLib.getIndexOfAddr vainparent fstLevel)
+              (VE {| pd := false; va := defautvaddr |}) (memory s) beqPage
+              beqIndex |}.
+
+Proof.
+
+set(s':= {|
+  currentPartition := currentPartition s;
+  memory := add ptVaInCurPart (StateLib.getIndexOfAddr vainparent fstLevel)
+              (VE {| pd := false; va := defautvaddr |}) (memory s) beqPage
+              beqIndex |}
+) in *.
+intros Hprops Hnotpart Hlookup (* Hnotderived *) Hnew1 Hnew2 Hcons .
+unfold propagatedPropertiesRemoveVaddr in *. intuition.
+  subst.
+  
+unfold consistency in *;intuition. 
+unfold physicalPageNotDerived in *.
+intros parent va  pdParent pageParent.
+intros Hparts HgetpdParent Hderiv Hmapparent child pdChild vaInChild pageChild
+Hgetchildren Hpdchild Hmapchild.
+assert(Hpartitions : getPartitions multiplexer s = getPartitions multiplexer s').
+symmetry.
+apply getPartitionsAddDerivation with entry ;trivial.
+rewrite Hpartitions in *.
+assert(Hchildren : 
+getChildren parent s' 
+   = getChildren parent s).
+apply getChildrenAddDerivation with entry;trivial.
+rewrite Hchildren in *;clear Hchildren.
+assert(Hgetpd: StateLib.getPd parent (memory s') =
+StateLib.getPd parent (memory s)). 
+apply getPdAddDerivation with entry;trivial.
+rewrite Hgetpd in *.
+assert(Hgetpdchild: StateLib.getPd child (memory s') =
+StateLib.getPd child (memory s)). 
+apply getPdAddDerivation with entry;trivial.
+rewrite Hgetpdchild in *. clear Hgetpdchild. clear Hgetpd.
+assert(Hmapped : forall pd v,  getMappedPage pd
+  s' v =
+getMappedPage pd s v).
+intros.
+apply getMappedPageAddDerivation with entry; trivial.
+rewrite Hmapped in *. clear Hmapped.
+assert (Hnewmapp : getMappedPage pdChildphy s vaChild = SomeDefault).
+{ 
+   apply getMappedPageNotPresent with ptVaChildpd phyDescChild;trivial.
+   intros;split; subst;trivial. }
+assert(Hor1:  
+((currentPartition s) = parent \/ (currentPartition s) <> parent)) by apply pageDecOrNot.
+destruct Hor1 as [Hor1| Hor1].
++ subst.
+  assert(Hor2 : checkVAddrsEqualityWOOffset nbLevel vainparent va level = true \/
+    checkVAddrsEqualityWOOffset nbLevel vainparent va level = false ).
+  { destruct (checkVAddrsEqualityWOOffset nbLevel vainparent va level);intuition. }
+  destruct Hor2 as [Hor2 | Hor2].
+  - assert(Hnewprop: exists pagetoremove, 
+  getAccessibleMappedPage currentPD s vainparent = SomePage  pagetoremove /\ 
+(forall child, In child (getChildren (currentPartition s) s) -> 
+~In  pagetoremove (getMappedPages child s)))by trivial.
+  destruct Hnewprop as (pg & Hpg & Hg1 ).
+  assert(pdParent = currentPD).
+  apply getPdNextEntryIsPPEq with (currentPartition s) s;trivial.
+  apply nextEntryIsPPgetPd;trivial.
+  apply nextEntryIsPPgetPd;trivial.
+  subst pdParent.
+  assert(Hpgmap: getMappedPage currentPD s vainparent = SomePage pg).
+  apply accessiblePAgeIsMapped;trivial.
+  assert(Hmapeq:  getMappedPage currentPD s vainparent =
+   getMappedPage currentPD s va).
+   apply getMappedPageEq with level;trivial.
+   symmetry;trivial.
+   rewrite Hmapparent in Hmapeq.
+   rewrite Hpgmap in Hmapeq.
+   inversion Hmapeq.
+   subst.
+  unfold not;intros;subst.
+  assert(Hgetchildreneq:In phyDescChild (getChildren (currentPartition s) s));
+  trivial.
+  generalize(Hg1 child Hgetchildren);clear Hg1;intros Hg1.
+  contradict Hg1.
+  unfold getMappedPages.
+  rewrite Hpdchild.
+  unfold getMappedPagesAux.
+  apply filterOptionInIff.
+  unfold getMappedPagesOption.
+  apply in_map_iff.
+  assert(Heqvars : exists va1, In va1 getAllVAddrWithOffset0 /\ 
+StateLib.checkVAddrsEqualityWOOffset nbLevel vaInChild va1 ( CLevel (nbLevel -1) ) = true )
+by apply AllVAddrWithOffset0.
+destruct Heqvars as (va1 & Hva1 & Hva11).
+exists va1;split;trivial.
+rewrite <- Hmapchild.
+symmetry.
+apply getMappedPageEq with level.
+symmetry;trivial.
+rewrite <- Hva11.
+f_equal.
+apply getNbLevelEq;trivial.
+ - apply Hcons with (currentPartition s) va pdParent child pdChild vaInChild;trivial.
+   
+unfold isDerived in *.
+unfold s' in *;simpl in *.
+clear s'.
+assert(Hgetsh1: StateLib.getFstShadow (currentPartition s) (add ptVaInCurPart (StateLib.getIndexOfAddr vainparent fstLevel)
+                (VE {| pd := false; va := defautvaddr |}) (memory s) beqPage
+                beqIndex)=
+StateLib.getFstShadow (currentPartition s) (memory s)). 
+apply getFstShadowAddDerivation with entry;trivial.
+rewrite Hgetsh1 in *. clear Hgetsh1.
+(* set(s':= {|
+  currentPartition := _ |}
+) in *. *)
+ case_eq (getFstShadow (currentPartition s) (memory s) );[intros sh1parent Hsh1parent | intros Hsh1parent];
+ rewrite Hsh1parent in *;trivial.
+ unfold not; intros Hgetvirt;
+ contradict Hderiv.
+
+ unfold getVirtualAddressSh1 in *.
+ assert(Hlevel:  StateLib.getNbLevel = Some level ) by (symmetry;trivial).
+ rewrite Hlevel in *.
+
+ rewrite getIndirectionAddDerivation with sh1parent ptVaInCurPart
+             (StateLib.getIndexOfAddr vainparent fstLevel)  defautvaddr s 
+ entry va level (nbLevel -1) false;
+ trivial.
+case_eq( getIndirection sh1parent va level (nbLevel - 1) s); 
+[intros ind Hind | intros Hind];
+ rewrite Hind in *;trivial.
+ case_eq(defaultPage =? ind);intros Heqind;rewrite Heqind in *;trivial.
+ simpl.
+ unfold StateLib.readVirEntry in *.
+ simpl in *.
+unfold consistency in *. 
+intuition.
+ assert(Hnotsameind : ind <> ptVaInCurPart \/ (StateLib.getIndexOfAddr va fstLevel) <>
+(StateLib.getIndexOfAddr vainparent fstLevel) ).
+{ apply pageTablesOrIndicesAreDifferent with sh1parent sh1parent level nbLevel s;trivial.
+apply sh1PartNotNull with (currentPartition s) s;trivial.
+apply nextEntryIsPPgetFstShadow;subst;trivial.
+apply sh1PartNotNull with (currentPartition s) s;trivial.
+apply nextEntryIsPPgetFstShadow;subst;trivial.
+  apply noDupConfigPagesListNoDupGetIndirections with (currentPartition s) sh1idx;trivial.
+  intuition.
+  right;left;trivial.
+  apply nextEntryIsPPgetFstShadow;subst;trivial.
+      apply noDupConfigPagesListNoDupGetIndirections with (currentPartition s) sh1idx;trivial.
+  intuition.
+  right;left;trivial.
+  apply nextEntryIsPPgetFstShadow;subst;trivial.
+  rewrite <- Hor2.
+  rewrite checkVAddrsEqualityWOOffsetPermut;trivial.
+  left;split;trivial.
+  apply getNbLevelEq;trivial.
+  symmetry;trivial.
+  apply beq_nat_false in Heqind.
+  unfold not; intros Htmp;subst;now contradict Heqind.
+  assert(Hnotnull : (defaultPage =? ptVaInCurPart) = false) by trivial.
+  apply beq_nat_false in Hnotnull.
+  unfold not; intros Htmp;subst;now contradict Hnotnull.
+  apply getIndirectionStopLevelGT  with (nbLevel - 1) ;trivial.
+  apply getNbLevelLt;intuition.
+  rewrite nbLevelEq.
+    symmetry. rewrite <- getNbLevelEq with level;trivial.
+    symmetry;trivial.
+assert(Haux :getIndirection sh1parent vainparent level (nbLevel -1) s = Some ptVaInCurPart). 
+  apply getIndirectionGetTableRoot with (currentPartition s);trivial.
+
+  intros.
+  split;subst;trivial.
+  apply getIndirectionStopLevelGT with (nbLevel - 1);trivial.
+    apply getNbLevelLt;intuition.
+  rewrite nbLevelEq.
+    symmetry. rewrite <- getNbLevelEq with level;trivial.
+    symmetry;trivial. }
+  
+(*   assert(Hreadpd :  StateLib.readPDflag ind (StateLib.getIndexOfAddr va fstLevel) (memory  {|
+              currentPartition := currentPartition s;
+              memory := add ptVaInCurPart
+                          (StateLib.getIndexOfAddr vainparent fstLevel)
+                          (VE {| pd := false; va := defautvaddr |})
+                          (memory s) beqPage beqIndex |})
+  = StateLib.readPDflag ind (StateLib.getIndexOfAddr va fstLevel) (memory s)).
+  apply readPDflagAddDerivation;trivial.
+    
+    rewrite Hreadpd;trivial.
+  assert(Hreadvir :  StateLib.readVirEntry ind (StateLib.getIndexOfAddr va fstLevel) (memory s')
+  = StateLib.readVirEntry ind (StateLib.getIndexOfAddr va fstLevel) (memory s)).
+  apply readVirEntryAddDerivation;trivial.
+  rewrite Hreadvir. split; trivial.  }
+ rewrite HgetPdflag.
+ rewrite Hgetvirt.
+ apply Hwell with partition pd;trivial. *)
+ assert(Htrue: beqPairs (ptVaInCurPart, StateLib.getIndexOfAddr vainparent fstLevel)
+        (ind, StateLib.getIndexOfAddr va fstLevel) beqPage beqIndex = false).
+ apply beqPairsFalse;intuition.
+ rewrite Htrue in *.
+ 
+ 
+ assert (lookup ind (StateLib.getIndexOfAddr va fstLevel)
+ (removeDup ptVaInCurPart (StateLib.getIndexOfAddr vainparent fstLevel)(memory s) beqPage beqIndex)
+           beqPage beqIndex = lookup  ind (StateLib.getIndexOfAddr va fstLevel) (memory s) beqPage beqIndex) as Hmemory.
+   { apply removeDupIdentity. intuition. }
+     rewrite Hmemory. trivial.
+     
+     + apply Hcons with parent va pdParent child pdChild vaInChild;trivial.
+     unfold isDerived in *.
+     assert(Hgetsh1: StateLib.getFstShadow parent (add ptVaInCurPart (StateLib.getIndexOfAddr vainparent fstLevel)
+                (VE {| pd := false; va := defautvaddr |}) (memory s) beqPage
+                beqIndex)=
+StateLib.getFstShadow parent (memory s)). 
+apply getFstShadowAddDerivation with entry;trivial.
+unfold s' in *. simpl in *.
+rewrite Hgetsh1 in *. clear Hgetsh1.
+(* set(s':= {|
+  currentPartition := _ |}
+) in *. *)
+ case_eq (getFstShadow parent (memory s) );[intros sh1parent Hsh1parent | intros Hsh1parent];
+ rewrite Hsh1parent in *;trivial.
+ unfold not; intros Hgetvirt;
+ contradict Hderiv.
+
+ unfold getVirtualAddressSh1 in *.
+ assert(Hlevel:  StateLib.getNbLevel = Some level ) by (symmetry;trivial).
+ rewrite Hlevel in *.
+
+(*  rewrite getIndirectionAddDerivation with sh1parent ptVaInCurPart
+             (StateLib.getIndexOfAddr vainparent fstLevel)  defautvaddr s 
+ entry va level (nbLevel -1) false;
+ trivial.
+case_eq( getIndirection sh1parent va level (nbLevel - 1) s); 
+[intros ind Hind | intros Hind];
+ rewrite Hind in *;trivial.
+ case_eq(defaultPage =? ind);intros Heqind;rewrite Heqind in *;trivial.
+ simpl.
+ unfold StateLib.readVirEntry in *.
+ simpl in *.
+unfold consistency in *. 
+intuition.
+ *)
+
+
+  assert(Hind :getIndirection sh1parent va level (nbLevel - 1)  {|
+      currentPartition := currentPartition s;
+      memory := add ptVaInCurPart
+                  (StateLib.getIndexOfAddr vainparent fstLevel)
+                  (VE {| pd := false; va := defautvaddr |}) (memory s)
+                  beqPage beqIndex |}
+  =getIndirection sh1parent va level (nbLevel - 1) s).
+  apply getIndirectionAddDerivation with entry;trivial.
+  rewrite Hind. clear Hind.
+  case_eq(getIndirection sh1parent va level (nbLevel - 1) s);
+  [intros ind Hind | intros Hind]; rewrite Hind in *;
+  trivial. 
+  
+  case_eq(ind =? defaultPage);intros Heqind.
+  assert(Hbof :  (defaultPage =? ind) = true).
+  { apply NPeano.Nat.eqb_eq.
+  apply beq_nat_true in Heqind.
+  subst;trivial.
+  destruct defaultPage;destruct ind;simpl in *;subst;trivial. }
+  rewrite Hbof in *;trivial.
+  assert(Hconfdif: configTablesAreDifferent s ) by (unfold consistency in *;intuition).
+assert(Hnotsameind : ind <> ptVaInCurPart).
+  {
+  assert(Hdist : Lib.disjoint (getConfigPages (currentPartition s) s)
+   (getConfigPages parent s)).
+  {  intuition.
+  rewrite <- Hpartitions in *.
+    apply Hconfdif;trivial. }
+  assert(Hin1 : In ind (getConfigPages parent s)).
+  { unfold getConfigPages.
+    simpl.
+    right.
+    apply inGetIndirectionsAuxInConfigPagesSh1 with sh1parent;trivial.
+    rewrite Hpartitions in *;trivial.
+    apply getIndirectionInGetIndirections with va level (nbLevel - 1);trivial. 
+    apply nbLevelNotZero.
+    
+    apply beq_nat_false in Heqind.
+    trivial.
+    unfold not;intros;subst; now contradict Heqind.
+    apply getNbLevelLe;trivial.
+    symmetry;trivial.
+    apply sh1PartNotNull with parent s;trivial.
+     rewrite Hpartitions in *;trivial.
+    apply nextEntryIsPPgetFstShadow;trivial. }
+  assert(Hin2 : In ptVaInCurPart (getConfigPages (currentPartition s) s)).
+  { apply isConfigTableSh1WithVE with vainparent;trivial.
+    intros;subst;split;intuition. }
+    unfold  Lib.disjoint in *.
+    unfold not in Hdist.
+    unfold not;intros Hfalse.
+    apply Hdist with  ptVaInCurPart;trivial.
+    subst;trivial. }
+    
+     assert(Hbof :  (defaultPage =? ind) = false).
+  { apply NPeano.Nat.eqb_neq.
+  apply beq_nat_false in Heqind.
+  subst;trivial.
+  destruct defaultPage;destruct ind;simpl in *;subst;trivial.
+  unfold not;intros;subst. now contradict Heqind. }
+  rewrite Hbof in *.
+  simpl.
+  
+  assert(Hreadpd :  StateLib.readVirEntry ind (StateLib.getIndexOfAddr va fstLevel) (memory s')
+  = StateLib.readVirEntry ind (StateLib.getIndexOfAddr va fstLevel) (memory s)).
+  apply readVirEntryAddDerivation;trivial.
+  left. 
+  
+    trivial.
+    unfold s' in *.
+    simpl in *.
+    rewrite Hreadpd .
+    trivial.
+    
+
+Qed. 
+
+
+Lemma consistencyRemoveVaddr s descChild vaChild currentPart level
+     idxDescChild ptDescChild currentPD ptDescChildFromPD idxDescChild1
+     phyDescChild pdChildphy idxvaChild ptVaChildpd shadow1Child
+     ptVaChildFromSh1 vainve sh2Childphy ptVaChildsh2 vainparent defautvaddr
+     currentShadow ptVaInCurPart idxvainparent: 
+(StateLib.getIndexOfAddr vainparent fstLevel) = idxvainparent -> 
+isPartitionFalse ptVaInCurPart
+              (StateLib.getIndexOfAddr vainparent fstLevel) s -> 
+   propagatedPropertiesRemoveVaddr s descChild vaChild currentPart level
+     idxDescChild ptDescChild currentPD ptDescChildFromPD idxDescChild1
+     phyDescChild pdChildphy idxvaChild ptVaChildpd shadow1Child
+     ptVaChildFromSh1 vainve sh2Childphy ptVaChildsh2 vainparent defautvaddr
+     currentShadow ptVaInCurPart (StateLib.getIndexOfAddr vainparent fstLevel) false
+     false ->
+     getPDFlag currentShadow vainparent s = false ->
+   (exists pagetoremove : page,
+      getAccessibleMappedPage currentPD s vainparent = SomePage pagetoremove /\
+      (forall child : page,
+       In child (getChildren currentPart s) ->
+       ~ In pagetoremove (getMappedPages child s)))
+       -> 
+consistency
+  {|
+  currentPartition := currentPartition s;
+  memory := add ptVaInCurPart (StateLib.getIndexOfAddr vainparent fstLevel)
+              (VE {| pd := false; va := defautvaddr |}) (memory s) beqPage
+              beqIndex |}. 
+Proof.
+intros;subst.
+unfold propagatedPropertiesRemoveVaddr in *.
+intuition.
+subst.
+assert(Hlookup :exists entry, 
+ lookup ptVaInCurPart (StateLib.getIndexOfAddr vainparent fstLevel) 
+ (memory s) beqPage beqIndex = Some (VE entry)).
+{ assert(Hva : isVE ptVaInCurPart (StateLib.getIndexOfAddr vainparent fstLevel) s) by intuition.
+
+  unfold isVE in *.
+
+ destruct(lookup ptVaInCurPart (StateLib.getIndexOfAddr vainparent fstLevel)
+          (memory s) beqPage beqIndex);intros; try now contradict Hva.
+ destruct v; try now contradict Hva.
+ do 2 f_equal.
+ exists v;trivial. }
+ destruct Hlookup as (entry & Hlookup).
+unfold consistency in *;intuition.
++ apply partitionDescriptorEntryAddDerivation with entry; intuition.
++ apply dataStructurePdSh1Sh2asRootAddDerivation with entry; intuition.
++ apply dataStructurePdSh1Sh2asRootAddDerivation with entry; intuition.
++ apply dataStructurePdSh1Sh2asRootAddDerivation with entry; intuition.
++ apply currentPartitionInPartitionsListAddDerivation with entry; intuition.
++ apply noDupMappedPagesListAddDerivation with entry; intuition.
++ apply noDupConfigPagesListAddDerivation with entry; intuition.
++ apply parentInPartitionListAddDerivation with entry; intuition.
++ apply accessibleVAIsNotPartitionDescriptorAddDerivation with entry; intuition.
++ apply accessibleChildPageIsAccessibleIntoParentAddDerivation with entry;intuition.
++ apply noCycleInPartitionTreeUpdtateSh1Structure with entry;intuition.
++ apply configTablesAreDifferentUpdtateSh1Structure with entry ;intuition.
++ apply isChildUpdtateSh1Structure with entry ;intuition.
++ apply isPresentNotDefaultIffAddDerivation ;intuition.
++ apply physicalPageNotDerivedRemoveVaddr with entry descChild
+vaChild (currentPartition s) level (StateLib.getIndexOfAddr descChild fstLevel) ptDescChild currentPD
+ptDescChildFromPD (StateLib.getIndexOfAddr descChild fstLevel) phyDescChild pdChildphy 
+(StateLib.getIndexOfAddr vaChild fstLevel)
+ptVaChildpd shadow1Child ptVaChildFromSh1 vainve sh2Childphy
+ptVaChildsh2 currentShadow;trivial. unfold propagatedPropertiesRemoveVaddr in *. 
+unfold consistency in *.
+intuition.  
++ apply multiplexerWithoutParentUpdtateSh1Structure with entry;intuition.
++ apply isParentUpdtateSh1Structure with entry;intuition.
++ apply noDupPartitionTreeUpdtateSh1Structure with entry;intuition.
++ apply wellFormedFstShadowUpdtateSh1Structure with entry ;intuition.
++ apply wellFormedSndShadowUpdtateSh1Structure with entry;intuition.
++ apply wellFormedShadowsUpdtateSh1Structure with entry;intuition.
++ apply wellFormedShadowsUpdtateSh1Structure with entry;intuition.
++ assert (Hprop: exists pagetoremove : page,
+       getAccessibleMappedPage currentPD s vainparent = SomePage pagetoremove /\
+       (forall child : page,
+        In child (getChildren (currentPartition s) s) ->
+        In pagetoremove (getMappedPages child s) -> False)) by trivial.
+  destruct Hprop as (x & Hx & Hxx).
+  rewrite nextEntryIsPPgetFstShadow in *.
+  assert(Hsh1cur: getFstShadow (currentPartition s) (memory s) = Some currentShadow);trivial.
+  unfold getAccessibleMappedPage in Hx.
+  assert(Hlevel :  Some level = StateLib.getNbLevel) by trivial.
+  rewrite <- Hlevel in *.
+  case_eq(getIndirection currentPD vainparent level (nbLevel - 1) s);
+  [intros ind Hind| intros Hind];rewrite Hind in *; try now contradict Hx.
+  case_eq(defaultPage =? ind);intros Hdef;rewrite Hdef in *;try now contradict Hx.
+  case_eq( StateLib.readPresent ind (StateLib.getIndexOfAddr vainparent fstLevel) (memory s));[intros pres Hpres|intros Hpres]; rewrite Hpres in *;try now contradict Hx.
+  case_eq pres;intros;subst;try now contradict Hx.
+  case_eq(  StateLib.readAccessible ind
+         (StateLib.getIndexOfAddr vainparent fstLevel) (memory s));[intros access Haccess|intros Haccess]; rewrite Haccess in *;try now contradict Hx.
+  case_eq access;intros;subst;try now contradict Hx. 
+  case_eq(  StateLib.readPhyEntry ind
+         (StateLib.getIndexOfAddr vainparent fstLevel) (memory s));[intros read Hread|intros Hread]; rewrite Hread in *;try now contradict Hx.
+  inversion Hx;subst.
+ 
+(*   
+ assert( Hpde: partitionDescriptorEntry s) by trivial.
+ unfold partitionDescriptorEntry in *.
+ assert(Hsh1cur:     (exists entry : page,
+          nextEntryIsPP (currentPartition s) sh1idx entry s /\ entry <> defaultPage)).
+   apply Hpde;trivial.
+   right;left;trivial.
+  destruct Hsh1cur as currentShadow1 *)
+unfold StateLib.readPhyEntry in Hread.
+case_eq(lookup ind (StateLib.getIndexOfAddr vainparent fstLevel) (memory s)
+            beqPage beqIndex);[intros v Hlookupread|intros Hlookupread]; rewrite Hlookupread in *;try now contradict Hread.
+destruct v;try now contradict Hread.
+inversion Hread.
+subst.
+apply  wellFormedFstShadowIfNoneUpdtateSh1StructureX  with entry true level
+(pa p) ind currentPD;trivial.
+unfold isPE.
+rewrite Hlookupread;trivial.
+unfold getTableAddrRoot.
+split.
+left;trivial.
+intros.
+exists level;split;trivial.
+exists (level+1).
+split;trivial.
+assert(tableroot=currentPD).
+apply getPdNextEntryIsPPEq with (currentPartition s) s;trivial.
+apply nextEntryIsPPgetPd;trivial.
+subst tableroot.
+
+apply getIndirectionStopLevelGT with (nbLevel - 1);trivial.
+omega.
+ rewrite nbLevelEq.
+    symmetry. rewrite <- getNbLevelEq with level;trivial.
+ unfold isEntryPage.
+ rewrite Hlookupread;trivial.
+ unfold entryPresentFlag.
+ unfold StateLib.readPresent in Hpres.
+ rewrite Hlookupread in Hpres.
+ rewrite Hlookupread.
+ inversion Hpres.
+ subst;trivial.
++ assert (Hprop: exists pagetoremove : page,
+       getAccessibleMappedPage currentPD s vainparent = SomePage pagetoremove /\
+       (forall child : page,
+        In child (getChildren (currentPartition s) s) ->
+        In pagetoremove (getMappedPages child s) -> False)) by trivial.
+  destruct Hprop as (x & Hx & Hxx).
+  rewrite nextEntryIsPPgetFstShadow in *.
+  assert(Hsh1cur: getFstShadow (currentPartition s) (memory s) = Some currentShadow);trivial.
+  unfold getAccessibleMappedPage in Hx.
+  assert(Hlevel :  Some level = StateLib.getNbLevel) by trivial.
+  rewrite <- Hlevel in *.
+  case_eq(getIndirection currentPD vainparent level (nbLevel - 1) s);
+  [intros ind Hind| intros Hind];rewrite Hind in *; try now contradict Hx.
+  case_eq(defaultPage =? ind);intros Hdef;rewrite Hdef in *;try now contradict Hx.
+  case_eq( StateLib.readPresent ind (StateLib.getIndexOfAddr vainparent fstLevel) (memory s));[intros pres Hpres|intros Hpres]; rewrite Hpres in *;try now contradict Hx.
+  case_eq pres;intros;subst;try now contradict Hx.
+  case_eq(  StateLib.readAccessible ind
+         (StateLib.getIndexOfAddr vainparent fstLevel) (memory s));[intros access Haccess|intros Haccess]; rewrite Haccess in *;try now contradict Hx.
+  case_eq access;intros;subst;try now contradict Hx. 
+  case_eq(  StateLib.readPhyEntry ind
+         (StateLib.getIndexOfAddr vainparent fstLevel) (memory s));[intros read Hread|intros Hread]; rewrite Hread in *;try now contradict Hx.
+  inversion Hx;subst.
+ 
+(*   
+ assert( Hpde: partitionDescriptorEntry s) by trivial.
+ unfold partitionDescriptorEntry in *.
+ assert(Hsh1cur:     (exists entry : page,
+          nextEntryIsPP (currentPartition s) sh1idx entry s /\ entry <> defaultPage)).
+   apply Hpde;trivial.
+   right;left;trivial.
+  destruct Hsh1cur as currentShadow1 *)
+unfold StateLib.readPhyEntry in Hread.
+case_eq(lookup ind (StateLib.getIndexOfAddr vainparent fstLevel) (memory s)
+            beqPage beqIndex);[intros v Hlookupread|intros Hlookupread]; rewrite Hlookupread in *;try now contradict Hread.
+destruct v;try now contradict Hread.
+inversion Hread.
+subst.
+apply  wellFormedFstShadowIfDefaultValuesUpdtateSh1StructureX  with entry true level
+(pa p) ind currentPD;trivial.
+unfold isPE.
+rewrite Hlookupread;trivial.
+unfold getTableAddrRoot.
+split.
+left;trivial.
+intros.
+exists level;split;trivial.
+exists (level+1).
+split;trivial.
+assert(tableroot=currentPD).
+apply getPdNextEntryIsPPEq with (currentPartition s) s;trivial.
+apply nextEntryIsPPgetPd;trivial.
+subst tableroot.
+
+apply getIndirectionStopLevelGT with (nbLevel - 1);trivial.
+omega.
+ rewrite nbLevelEq.
+    symmetry. rewrite <- getNbLevelEq with level;trivial.
+ unfold isEntryPage.
+ rewrite Hlookupread;trivial.
+ unfold entryPresentFlag.
+ unfold StateLib.readPresent in Hpres.
+ rewrite Hlookupread in Hpres.
+ rewrite Hlookupread.
+ inversion Hpres.
+ subst;trivial.
+Qed.
+
+
+Lemma writeVirEntryRemoveVaddr  descChild vaChild currentPart level
+     idxDescChild ptDescChild currentPD ptDescChildFromPD idxDescChild1
+     phyDescChild pdChildphy idxvaChild ptVaChildpd shadow1Child
+     ptVaChildFromSh1 vainve sh2Childphy ptVaChildsh2 vainparent defautvaddr
+     currentShadow ptVaInCurPart idxvainparent: 
+
+{{ fun s : state =>
+   propagatedPropertiesRemoveVaddr s descChild vaChild currentPart level
+     idxDescChild ptDescChild currentPD ptDescChildFromPD idxDescChild1
+     phyDescChild pdChildphy idxvaChild ptVaChildpd shadow1Child
+     ptVaChildFromSh1 vainve sh2Childphy ptVaChildsh2 vainparent defautvaddr
+     currentShadow ptVaInCurPart idxvainparent false
+     false /\  getPDFlag currentShadow vainparent s = false /\
+   (exists pagetoremove : page,
+      getAccessibleMappedPage currentPD s vainparent = SomePage pagetoremove /\
+      (forall child : page,
+       In child (getChildren currentPart s) ->
+       ~ In pagetoremove (getMappedPages child s)))}} 
+  MAL.writeVirEntry ptVaInCurPart idxvainparent defautvaddr {{ fun (_ : unit) (s : state) =>
+                       partitionsIsolation s /\
+                       kernelDataIsolation s /\
+                       verticalSharing s /\ consistency s }}.
+Proof.
+intros.
+subst.
+eapply weaken.
+eapply WP.writeVirEntry.
+simpl;intros.
+unfold propagatedPropertiesRemoveVaddr in *.
+assert (Hve :isVE ptVaInCurPart idxvainparent s)
+  by (intuition;subst;trivial).
+unfold isVE in Hve.
+case_eq( lookup ptVaInCurPart idxvainparent (memory s) beqPage beqIndex);
+intros; rewrite H0 in *; try now contradict Hve.
+case_eq v ; intros;rewrite H1 in *; try now contradict Hve.
+subst.
+assert(Hparts : In currentPart (getPartitions multiplexer s)).
+{ intuition. subst.
+  unfold consistency in *.
+  unfold currentPartitionInPartitionsList in *.
+  intuition. }
+assert(Hcursh1 :(exists entry : page,
+        nextEntryIsPP currentPart sh1idx entry s /\ entry <> defaultPage)).
+{ assert(Hpde: partitionDescriptorEntry s) by (unfold consistency in *;intuition).
+  apply Hpde;intuition.   }
+destruct Hcursh1 as (currentShadow1 & Hcursh1 & Hsh1notnul). 
+assert (Hreadflag : isPartitionFalse ptVaInCurPart (StateLib.getIndexOfAddr vainparent fstLevel) s ).
+{ unfold isPartitionFalse.
+unfold consistency in *. 
+assert(Haccessva : accessibleVAIsNotPartitionDescriptor s) by intuition.
+unfold accessibleVAIsNotPartitionDescriptor in *.
+
+assert (Hflag : getPDFlag currentShadow vainparent s = false).
+intuition;subst.
+ trivial.
+apply getPDFlagReadPDflag  with currentShadow vainparent currentPart; trivial.
+intuition.  
+apply Nat.eqb_neq.
+assert(Hfalsepge : (defaultPage =? ptVaInCurPart) = false) by trivial.
+apply beq_nat_false in Hfalsepge.
+unfold not;intros Hfalse'.
+rewrite Hfalse' in Hfalsepge.    
+now contradict Hfalsepge.
+intuition.
+intuition.
+intuition.
+subst;trivial. }
+assert(StateLib.getIndexOfAddr vainparent fstLevel = idxvainparent) by
+intuition.
+subst.
+intuition try assumption. 
++ apply partitionsIsolationUpdtateSh1Structure with v0; trivial.
++ apply kernelDataIsolationUpdtateSh1Structure with v0;trivial.
++ apply verticalSharingUpdtateSh1Structure with v0;trivial.
++ apply consistencyRemoveVaddr with descChild
+vaChild (currentPartition s) level (StateLib.getIndexOfAddr descChild fstLevel) ptDescChild currentPD
+ptDescChildFromPD (StateLib.getIndexOfAddr descChild fstLevel) phyDescChild pdChildphy 
+(StateLib.getIndexOfAddr vaChild fstLevel)
+ptVaChildpd shadow1Child ptVaChildFromSh1 vainve sh2Childphy
+ptVaChildsh2 currentShadow (StateLib.getIndexOfAddr vainparent fstLevel);trivial.
+
+unfold propagatedPropertiesRemoveVaddr. 
+subst.
+intuition.
+unfold not.
+subst. 
+trivial. 
+Qed. 
+
 
 
 
